proofs/lean/infinite_tables/safe_table_select_revision/lakefile.lean
@@ -7,7 +7,8 @@ package «safe_table_select_revision» where
     ⟨`relaxedAutoImplicit, false⟩
   ]
 
-require mathlib from "../../../../../deps/mathlib4"
+require mathlib from git
+  "https://github.com/leanprover-community/mathlib4.git" @ "v4.25.0-rc2"
 
 @[default_target]
 lean_lib Proofs
